p256: prove ecdsa-verify

code/ecdsap256/Hacl.Impl.P256.Verify.fst
@@ -16,6 +16,7 @@ open Hacl.Impl.P256.PointMul
 module BSeq = Lib.ByteSequence
 
 module S = Spec.P256
+module SL = Spec.P256.Lemmas
 module SM = Hacl.Spec.P256.Montgomery
 module QI = Hacl.Impl.P256.Qinv
 
@@ -77,45 +78,60 @@ let ecdsa_verification_get_u12 u1 u2 r s z =
 
 
 inline_for_extraction noextract
-val ecdsa_verification_getx: x:felem -> pk:point -> u1:felem -> u2:felem -> Stack bool
+val ecdsa_verify_finv: p:point -> r:felem -> Stack bool
   (requires fun h ->
-    live h x /\ live h pk /\ live h u1 /\ live h u2 /\
-    disjoint x u1 /\ disjoint x u2 /\ disjoint x pk /\
-    disjoint pk u1 /\ disjoint pk u2 /\
-    point_inv h pk /\ as_nat h u1 < S.order /\ as_nat h u2 < S.order)
-  (ensures fun h0 b h1 -> modifies (loc x) h0 h1 /\
-   (let res_proj =
-     S.point_mul_double_g (as_nat h0 u1) (as_nat h0 u2) (from_mont_point (as_point_nat h0 pk)) in
-    let (rx, _) = S.to_aff_point res_proj in
-    b == not (S.is_point_at_inf res_proj) /\ as_nat h1 x == rx % S.order))
+    live h p /\ live h r /\ disjoint p r /\
+    point_inv h p /\ 0 < as_nat h r /\ as_nat h r < S.order)
+    //not (S.is_point_at_inf (from_mont_point (as_point_nat h p))))
+  (ensures  fun h0 b h1 -> modifies0 h0 h1 /\
+    (let (_X, _Y, _Z) = from_mont_point (as_point_nat h0 p) in
+     b <==> (S.fmul _X (S.finv _Z) % S.order = as_nat h0 r)))
 
-let ecdsa_verification_getx x pk u1 u2 =
+let ecdsa_verify_finv p r_q =
   push_frame ();
-  let res_proj = create_point () in
+  let x = create_felem () in
+  to_aff_point_x x p;
+  qmod_short x x;
+  let res = bn_is_eq_vartime4 x r_q in
+  pop_frame ();
+  res
+
+
+inline_for_extraction noextract
+val ecdsa_verification_cmpr: r:felem -> pk:point -> u1:felem -> u2:felem -> Stack bool
+  (requires fun h ->
+    live h r /\ live h pk /\ live h u1 /\ live h u2 /\
+    disjoint r u1 /\ disjoint r u2 /\ disjoint r pk /\
+    disjoint pk u1 /\ disjoint pk u2 /\
+    point_inv h pk /\ as_nat h u1 < S.order /\ as_nat h u2 < S.order /\
+    0 < as_nat h r /\ as_nat h r < S.order)
+  (ensures fun h0 b h1 -> modifies0 h0 h1 /\
+    (let _X, _Y, _Z = S.point_mul_double_g (as_nat h0 u1) (as_nat h0 u2)
+      (from_mont_point (as_point_nat h0 pk)) in
+    b <==> (if S.is_point_at_inf (_X, _Y, _Z) then false
+      else S.fmul _X (S.finv _Z) % S.order = as_nat h0 r)))
+
+let ecdsa_verification_cmpr r pk u1 u2 =
+  push_frame ();
+  let res = create_point () in
   let h0 = ST.get () in
-  point_mul_double_g res_proj u1 u2 pk;
+  point_mul_double_g res u1 u2 pk;
   let h1 = ST.get () in
-  assert (S.to_aff_point (from_mont_point (as_point_nat h1 res_proj)) ==
+  assert (S.to_aff_point (from_mont_point (as_point_nat h1 res)) ==
     S.to_aff_point (S.point_mul_double_g (as_nat h0 u1) (as_nat h0 u2)
       (from_mont_point (as_point_nat h0 pk))));
-  let is_res_point_at_inf = is_point_at_inf_vartime res_proj in
-  //assert (is_res_point_at_inf == S.is_point_at_inf
-    //(from_mont_point (as_point_nat h1 res_proj)));
-  assume (is_res_point_at_inf == S.is_point_at_inf
-    (S.point_mul_double_g (as_nat h0 u1) (as_nat h0 u2) (from_mont_point (as_point_nat h0 pk))));
 
-  to_aff_point_x x res_proj;
-  let h2 = ST.get () in
-  qmod_short x x;
-  let h3 = ST.get () in
-  assert (as_nat h2 x == fst (S.to_aff_point
-    (S.point_mul_double_g (as_nat h0 u1) (as_nat h0 u2) (from_mont_point (as_point_nat h0 pk)))));
-  assert (as_nat h3 x == as_nat h2 x % S.order);
+  SL.lemma_aff_is_point_at_inf (from_mont_point (as_point_nat h1 res));
+  SL.lemma_aff_is_point_at_inf
+    (S.point_mul_double_g (as_nat h0 u1) (as_nat h0 u2) (from_mont_point (as_point_nat h0 pk)));
+
+  let b =
+    if is_point_at_inf_vartime res then false
+    else ecdsa_verify_finv res r in
   pop_frame ();
-  not is_res_point_at_inf
+  b
 
 
-// TODO: use variable time cmp with scalar
 inline_for_extraction noextract
 val load_signature (r_q s_q:felem) (sign_r sign_s:lbytes 32ul) : Stack bool
   (requires fun h ->
@@ -153,23 +169,20 @@ val ecdsa_verify_msg_as_qelem:
 [@CInline]
 let ecdsa_verify_msg_as_qelem m_q public_key signature_r signature_s =
   push_frame ();
-  let tmp = create 32ul (u64 0) in
+  let tmp = create 28ul (u64 0) in
   let pk  = sub tmp 0ul 12ul in
   let r_q = sub tmp 12ul 4ul in
   let s_q = sub tmp 16ul 4ul in
   let u1  = sub tmp 20ul 4ul in
   let u2  = sub tmp 24ul 4ul in
-  let x   = sub tmp 28ul 4ul in
 
   let is_pk_valid = load_point_vartime pk public_key in
   let is_rs_valid = load_signature r_q s_q signature_r signature_s in
 
-  if not (is_pk_valid && is_rs_valid) then
-    begin pop_frame (); false end
-  else begin
-    ecdsa_verification_get_u12 u1 u2 r_q s_q m_q;
-    let b = ecdsa_verification_getx x pk u1 u2 in
-    if not b then
-      begin pop_frame (); false end
-      else
-        begin let res = bn_is_eq_vartime4 x r_q in pop_frame (); res end end
+  let res =
+    if not (is_pk_valid && is_rs_valid) then false
+    else begin
+      ecdsa_verification_get_u12 u1 u2 r_q s_q m_q;
+      ecdsa_verification_cmpr r_q pk u1 u2 end in
+  pop_frame ();
+  res
