specs/lemmas/Spec.P256.Lemmas.fst
@@ -3,9 +3,18 @@ module Spec.P256.Lemmas
 open FStar.Mul
 open Spec.P256.PointOps
 
+module M = Lib.NatMod
+
 #set-options "--z3rlimit 50 --ifuel 0 --fuel 0"
 
 let prime_lemma () = admit()
+
+let lemma_aff_is_point_at_inf p =
+  prime_lemma ();
+  let (px, py, pz) = p in
+  M.lemma_div_mod_prime_is_zero #prime px pz;
+  M.lemma_div_mod_prime_is_zero #prime py pz
+
 
 let aff_point_at_inf_lemma p = admit()
 
